\documentclass[12pt]{article}

\usepackage{amsmath}
\usepackage[margin=0.75in]{geometry}
\usepackage[numbers]{natbib}
\usepackage{physics}
\usepackage[hyphens]{url}
\usepackage[labelformat=simple,position=b]{subcaption}
\renewcommand\thesubfigure{(\alph{subfigure})}
\usepackage{fancyhdr}
\pagestyle{fancy}
\fancyhf{}
\rhead{cosmiQ}
\lhead{Hackathon 2021}
\rfoot{Page \thepage}

\usepackage{graphicx}
\graphicspath{
	{figures}
}

\usepackage[hidelinks]{hyperref}


\renewcommand{\phi}{\varphi}


\title{Hackathon Docs}
\author{cosmiQ}
\date{\today}

\begin{document}

\maketitle

%\thispagestyle{empty}
\section*{Introduction}

\section*{Task 1}

\section*{Task 2}

\begin{align}
\hat{D} &= \sum_{t_0}^{t_f-1} \sum_i -\mu(t,i) \left[ \frac{1}{K}\sum_{q=0}^{N_q-1} d^q \hat{n}(i,t,q) \right]
+ \frac{\gamma}{2}\sum_{t=t_0}^{t_f-1} \sum_{ij} \Sigma^t_{ij} \left[ \frac{1}{K} \sum_{q=0}^{N_q-1} d^q \hat{n}(i,t,q) \right] \left[ \frac{1}{K} \sum_{\bar{q}=0}^{N_q-1} d^q \hat{n}(j,t,\bar{q}) \right] \nonumber\\
&+ \sum_{t_0}^{t_f-1} \sum_{ij} \lambda(t,i)\lambda(t,j) \Bigg\{ \left[ \frac{1}{K} \sum_{q=0}^{N_q-1} d^q \hat{n}(j,t+1,q) \right]\left[ \frac{1}{K} \sum_{q=0}^{N_q-1} d^q \hat{n}(i,t+1,q) \right] \nonumber\\ 
&-2\left[ \frac{1}{K} \sum_{q=0}^{N_q-1} d^q \hat{n}(i,t+1,q) \right]\left[ \frac{1}{K} \sum_{q=0}^{N_q-1} d^q \hat{n}(j,t,q)\right] +\left[ \frac{1}{K} \sum_{q=0}^{N_q-1} d^q \hat{n}(i,t,q) \right] \left[ \frac{1}{K} \sum_{q=0}^{N_q-1} d^q \hat{n}(j,t,q) \right] \Bigg\} \nonumber\\
&+ \rho \sum_{t_0}^{t_f} \sum_{ij} \left[ \frac{1}{K} \sum_{q=0}^{N_q-1} d^q \hat{n}(i,t,q) \right] \left[ \frac{1}{K} \sum_{\bar{q}=0}^{N_q-1} d^q \hat{n}(j,t,\bar{q}) \right] 
-2\rho \sum_{t_0}^{t_f} \sum_{i} \left[ \frac{1}{K} \sum_{q=0}^{N_q-1} d^q \hat{n}(i,t,q) \right] + N_t\cdot N^2
\end{align}

Which we may further simplify by collecting terms:
\begin{align}
K\hat{D} &= \sum_{t_0}^{t_f-1} \sum_i \sum_{q=0}^{N_q-1} (-\mu(t,i) - 2\rho) d^q \hat{n}(i,t,q) \nonumber\\
&+ \frac{1}{K} \sum_{t_0}^{t_f-1} \sum_{ij} \sum_{q=0}^{N_q-1}\sum_{\bar{q}=0}^{N_q-1} \left[ \frac{\gamma}{2}{\Sigma^t_{ij}} + \lambda(t,i)\lambda(t,j) + \rho \right] d^q \hat{n}(i,t,q) d^q \hat{n}(j,t,\bar{q}) \nonumber\\
&+ \frac{1}{K} \sum_{t_0}^{t_f-1} \sum_{ij} \sum_{q=0}^{N_q-1}\sum_{\bar{q}=0}^{N_q-1} \lambda(t,i)\lambda(t,j) \left[ d^q \hat{n}(i,t+1,q) d^q \hat{n}(j,t+1,\bar{q}) - 2 d^q \hat{n}(i,t+1,q) d^q \hat{n}(j,t,\bar{q}) \right] \nonumber\\    
&+\frac{\rho}{K}  \sum_{ij} \sum_{q=0}^{N_q-1}\sum_{\bar{q}=0}^{N_q-1} d^q \hat{n}(i,t_f,q) d^q \hat{n}(j,t_f,\bar{q}) - 2\rho \sum_i \sum_{q=0}^{N_q-1} d^q \hat{n}(i,t_f,q) \nonumber\\
&+ K\cdot N_t\cdot N^2 
\end{align}

Note that while the boundary term contributes to the inner Hamiltonian, it only appears as a separate term due to the constraint. We have no information available about relative profits ($\mu(i,t_f)$), risk ($\Sigma^{t_f}_{ij}$), and transaction cost ($\lambda(t,i)$) at the final time $t = t_f$.\\

Using $\mu(t_f,i) = 0$ and $\Sigma^{t_f} = 0$, a more compressed notation gives us:
\begin{align}
K\hat{D} &= \sum_{t_0}^{t_f} \sum_i \sum_{q=0}^{N_q-1} (-\mu(t,i) - 2\rho) d^q \hat{n}(i,t,q) \nonumber\\
&+ \frac{1}{K} \sum_{t_0}^{t_f} \sum_{i<j} \sum_{q=0}^{N_q-1}\sum_{\bar{q}=0}^{N_q-1} 2\left[ \frac{\gamma}{2} {\Sigma^t_{ij}} + \lambda(t,i)\lambda(t,j) + \rho \right] d^q \hat{n}(i,t,q) d^q \hat{n}(j,t,\bar{q}) \nonumber\\
&+ \frac{1}{K} \sum_{t_0}^{t_f} \sum_{i} \sum_{q=0}^{N_q-1}\sum_{\bar{q}=0}^{N_q-1} \left[ \frac{\gamma}{2} {\Sigma^t_{ii}} + \lambda(t,i)\lambda(t,i) + \rho \right] d^q \hat{n}(i,t,q) d^q \hat{n}(i,t,\bar{q}) \nonumber\\
&+ \frac{1}{K} \sum_{t_0}^{t_f-1} \sum_{i<j} \sum_{q=0}^{N_q-1}\sum_{\bar{q}=0}^{N_q-1} 2\lambda(t,i)\lambda(t,j) \left[ d^q \hat{n}(i,t+1,q) d^q \hat{n}(j,t+1,\bar{q}) - 2 d^q \hat{n}(i,t+1,q) d^q \hat{n}(j,t,\bar{q}) \right] \nonumber\\    
&+ \frac{1}{K} \sum_{t_0}^{t_f-1} \sum_{i} \sum_{q=0}^{N_q-1}\sum_{\bar{q}=0}^{N_q-1} 2\lambda(t,i)\lambda(t,i) \left[ d^q \hat{n}(i,t+1,q) d^q \hat{n}(i,t+1,\bar{q}) - 2 d^q \hat{n}(i,t+1,q) d^q \hat{n}(i,t,\bar{q}) \right] \nonumber\\    
&+ K\cdot N_t\cdot N^2 
\end{align}

For MPS we need to collect terms a little differently:
\begin{align}
%1
K\hat{D} &= \sum_{t_0}^{t_f} \sum_i \sum_{q=0}^{N_q-1} (-\mu(t,i) - 2\rho) d^q \hat{n}(i,t,q) \nonumber\\
%2
&+ \frac{1}{K} \sum_{t_0}^{t_f} \sum_{i<j} \sum_{q<\bar{q}}^{N_q-1} 4\left[ \frac{\gamma}{2} {\Sigma^t_{ij}} + \lambda(t,i)\lambda(t,j) + \rho \right] d^q \hat{n}(i,t,q) d^q \hat{n}(j,t,\bar{q}) \nonumber\\
%3
&+ \frac{1}{K} \sum_{t_0}^{t_f} \sum_{i<j} \sum_{q}^{N_q-1} 2\left[ \frac{\gamma}{2} {\Sigma^t_{ij}} + \lambda(t,i)\lambda(t,j) + \rho \right] d^q \hat{n}(i,t,q) d^q \hat{n}(j,t,q) \nonumber\\
%4
&+ \frac{1}{K} \sum_{t_0}^{t_f} \sum_{i} \sum_{q<\bar{q}}^{N_q-1} 2\left[ \frac{\gamma}{2} {\Sigma^t_{ii}} + \lambda(t,i)\lambda(t,i) + \rho \right] d^q \hat{n}(i,t,q) d^q \hat{n}(i,t,\bar{q}) \nonumber\\
%5
&+ \frac{1}{K} \sum_{t_0}^{t_f} \sum_{i} \sum_{q=0}^{N_q-1} \left[ \frac{\gamma}{2} {\Sigma^t_{ii}} + \lambda(t,i)\lambda(t,i) + \rho \right] d^q \hat{n}(i,t,q) d^q \hat{n}(i,t,{q}) \nonumber\\
%6
&+ \frac{1}{K} \sum_{t_0}^{t_f-1} \sum_{i<j} \sum_{q<\bar{q}}^{N_q-1} 4\lambda(t,i)\lambda(t,j) \left[ d^q \hat{n}(i,t+1,q) d^q \hat{n}(j,t+1,\bar{q}) - 2 d^q \hat{n}(i,t+1,q) d^q \hat{n}(j,t,\bar{q}) \right] \nonumber\\    
%7
&+ \frac{1}{K} \sum_{t_0}^{t_f-1} \sum_{i<j} \sum_{q=0}^{N_q-1} 2\lambda(t,i)\lambda(t,j) \left[ d^q \hat{n}(i,t+1,q) d^q \hat{n}(j,t+1,{q}) - 2 d^q \hat{n}(i,t+1,q) d^q \hat{n}(j,t,{q}) \right] \nonumber\\    
%8
&+ \frac{1}{K} \sum_{t_0}^{t_f-1} \sum_{i} \sum_{q<\bar{q}}^{N_q-1}4\lambda(t,i)\lambda(t,i) \left[ d^q \hat{n}(i,t+1,q) d^q \hat{n}(i,t+1,\bar{q}) - 2 d^q \hat{n}(i,t+1,q) d^q \hat{n}(i,t,\bar{q}) \right] \nonumber\\    
%9
&+ \frac{1}{K} \sum_{t_0}^{t_f-1} \sum_{i} \sum_{q=0}^{N_q-1} 2\lambda(t,i)\lambda(t,i) \left[ d^q \hat{n}(i,t+1,q) d^q \hat{n}(i,t+1,{q}) - 2 d^q \hat{n}(i,t+1,q) d^q \hat{n}(i,t,{q}) \right] \nonumber\\ 
%10
&+ K\cdot N_t\cdot N^2 
\end{align}

And we rearrange to have all the on-site pieces together:
\begin{align}
%1
K\hat{D} &= \sum_{t_0}^{t_f} \sum_i \sum_{q=0}^{N_q-1} (-\mu(t,i) - 2\rho) d^q \hat{n}(i,t,q) \nonumber\\
%2
&+ \frac{1}{K} \sum_{t_0}^{t_f} \sum_{i} \sum_{q=0}^{N_q-1} \left[ \frac{\gamma}{2} {\Sigma^t_{ii}} + \lambda(t,i)\lambda(t,i) + \rho \right] d^q \hat{n}(i,t,q) d^q \hat{n}(i,t,{q}) \nonumber\\
%3
&+ \frac{1}{K} \sum_{t_0 = 1}^{t_f} \sum_{i} \sum_{q=0}^{N_q-1} 2\lambda(t-1,i)\lambda(t-1,i) d^q \hat{n}(i,t,q) d^q \hat{n}(i,t,{q}) \nonumber\\ 
%
%
%4
&+ \frac{1}{K} \sum_{t_0}^{t_f} \sum_{i} \sum_{q<\bar{q}}^{N_q-1} 2\left[ \frac{\gamma}{2} {\Sigma^t_{ii}} + \lambda(t,i)\lambda(t,i) + \rho \right] d^q \hat{n}(i,t,q) d^q \hat{n}(i,t,\bar{q}) \nonumber\\
%
%
%
%8
&+ \frac{1}{K} \sum_{t_0}^{t_f-1} \sum_{i} \sum_{q<\bar{q}}^{N_q-1}4\lambda(t,i)\lambda(t,i) \left[ d^q \hat{n}(i,t+1,q) d^q \hat{n}(i,t+1,\bar{q}) - 2 d^q \hat{n}(i,t+1,q) d^q \hat{n}(i,t,\bar{q}) \right] \nonumber\\    
%2
&+ \frac{1}{K} \sum_{t_0}^{t_f} \sum_{i<j} \sum_{q<\bar{q}}^{N_q-1} 4\left[ \frac{\gamma}{2} {\Sigma^t_{ij}} + \lambda(t,i)\lambda(t,j) + \rho \right] d^q \hat{n}(i,t,q) d^q \hat{n}(j,t,\bar{q}) \nonumber\\
%3
&+ \frac{1}{K} \sum_{t_0}^{t_f} \sum_{i<j} \sum_{q}^{N_q-1} 2\left[ \frac{\gamma}{2} {\Sigma^t_{ij}} + \lambda(t,i)\lambda(t,j) + \rho \right] d^q \hat{n}(i,t,q) d^q \hat{n}(j,t,q) \nonumber\\
%6
&+ \frac{1}{K} \sum_{t_0}^{t_f-1} \sum_{i<j} \sum_{q<\bar{q}}^{N_q-1} 4\lambda(t,i)\lambda(t,j) \left[ d^q \hat{n}(i,t+1,q) d^q \hat{n}(j,t+1,\bar{q}) - 2 d^q \hat{n}(i,t+1,q) d^q \hat{n}(j,t,\bar{q}) \right] \nonumber\\    
%7
&+ \frac{1}{K} \sum_{t_0}^{t_f-1} \sum_{i<j} \sum_{q=0}^{N_q-1} 2\lambda(t,i)\lambda(t,j) \left[ d^q \hat{n}(i,t+1,q) d^q \hat{n}(j,t+1,{q}) - 2 d^q \hat{n}(i,t+1,q) d^q \hat{n}(j,t,{q}) \right] \nonumber\\    
%9b
&+ \frac{1}{K} \sum_{t_0}^{t_f-1} \sum_{i} \sum_{q=0}^{N_q-1} 2\lambda(t,i)\lambda(t,i) \left[ - 2 d^q \hat{n}(i,t+1,q) d^q \hat{n}(i,t,{q}) \right] \nonumber\\ 
%10
&+ K\cdot N_t\cdot N^2 
\end{align}


\begin{thebibliography}{10}
\end{thebibliography}

\end{document}
